examples/tactics/StringPrinterTest.fst
@@ -4,8 +4,16 @@ module U32 = FStar.UInt32
 module HST = FStar.HyperStack.ST
 module B = FStar.Buffer
 module SP = StringPrinterTest.Aux
+module U8 = FStar.UInt8
+module HS = FStar.HyperStack
 
-let test3 (x: U32.t) : HST.ST (option unit) (requires (fun _ -> True)) (ensures (fun h _ h' -> B.modifies_0 h h')) =
-  SP.example_test x
+let test3 (x: U32.t) : HST.ST (option (B.buffer U8.t))
+  (requires (fun _ -> True))
+  (ensures (fun h res h' ->
+    match res with
+    | None -> h' == h
+    | Some b -> SP.buffer_create_mm_post HS.root h h' b
+  ))
+= SP.example_test x
 
 // krml -tmpdir ou -bundle 'StringPrinter.\*' -bundle StringPrinterTest.Aux -drop 'FStar.Tactics.\*' -drop 'FStar.Reflection.\*' StringPrinterTest.fst -skip-linking
